brought in new BucketsLib

lib/Buckets/BucketsLib.i.dfy
@@ -4,6 +4,7 @@ include "../Base/Maps.s.dfy"
 include "../Base/total_order.i.dfy"
 include "../../MapSpec/UI.s.dfy"
 include "../../MapSpec/MapSpec.s.dfy"
+
 //
 // A Bucket maps keys to Messages. A BucketList imparts a Message meaning
 // to every key obeying the Message composition rules. This module shows
@@ -23,21 +24,29 @@ module BucketsLib {
   import MS = MapSpec
 
   type BucketMap = map<Key, Message>
-    // TODO(jonh): The Bucket datatype is denormalized and has two
-    // representations of the same data.  Should do this with a
-    // function view of the same data.
   datatype Bucket = BucketMapWithSeq(b: BucketMap, keys: seq<Key>, msgs: seq<Message>)
   type BucketList = seq<Bucket>
 
-  function BucketMapOfSeq(keys: seq<Key>, msgs: seq<Message>) : BucketMap
-  requires |keys| == |msgs|
-
+  function {:opaque} BucketMapOfSeq(keys: seq<Key>, msgs: seq<Message>) : (result: BucketMap)
+    requires |keys| == |msgs|
+    ensures result.Keys == Set(keys)
+    ensures result.Values <= Set(msgs)
+  {
+    if |keys| == 0 then
+      map[]
+    else
+      var r' := BucketMapOfSeq(DropLast(keys), DropLast(msgs));
+      var r := r'[Last(keys) := Last(msgs)];
+      assert r.Values <= r'.Values + {Last(msgs)};
+      r
+  }
+  
   predicate WFBucketMap(bucket: BucketMap)
   {
     forall key | key in bucket :: bucket[key] != IdentityMessage()
   }
 
-  predicate {:opaque} WFBucket(bucket: Bucket)
+  predicate WFBucket(bucket: Bucket)
   {
     && WFBucketMap(bucket.b)
     && |bucket.keys| == |bucket.msgs|
@@ -46,7 +55,7 @@ module BucketsLib {
 
   predicate BucketWellMarshalled(bucket: Bucket)
   {
-    Lexicographic_Byte_Order.IsStrictlySorted(bucket.keys)
+    IsStrictlySorted(bucket.keys)
   }
 
   predicate BucketListWellMarshalled(blist: BucketList)
@@ -54,10 +63,120 @@ module BucketsLib {
     forall i | 0 <= i < |blist| :: BucketWellMarshalled(blist[i])
   }
 
-  function B(m: BucketMap) : (bucket: Bucket)
+  function BInternal(m: BucketMap) : (bucket: Bucket)
+    ensures bucket.b == m
+    ensures |bucket.keys| == |bucket.msgs|
+  {
+    if |m.Keys| == 0 then
+      BucketMapWithSeq(m, [], [])
+    else 
+      var maxkey := maximum(m.Keys);
+      var maxmsg := m[maxkey];
+      var subm := MapRemove1(m, maxkey);
+      var subbucket := BInternal(subm);
+      BucketMapWithSeq(m, subbucket.keys + [maxkey], subbucket.msgs + [maxmsg])
+  }
+
+  lemma BInternalWellMarshalled(m: BucketMap)
+  ensures BucketWellMarshalled(BInternal(m))
+  //ensures WFBucketMap(m) ==> WFBucket(BInternal(m))
+  {
+    if |m| == 0 {
+      reveal_IsStrictlySorted();
+    } else if |m| == 1 {
+      reveal_IsStrictlySorted();
+    } else {
+      var maxkey := maximum(m.Keys);
+      var subm := MapRemove1(m, maxkey);
+      var subbucket := BInternal(subm);      
+      BInternalWellMarshalled(subm);
+      StrictlySortedAugment(subbucket.keys, maxkey);
+    }
+  }
+  
+  lemma BInternalWFBucket(m: BucketMap)
+    requires WFBucketMap(m)
+    ensures WFBucket(BInternal(m))
+  {
+    // reveal_WFBucket();
+    reveal_BucketMapOfSeq();
+  }
+
+  function {:opaque} B(m: BucketMap) : (bucket: Bucket)
   ensures bucket.b == m
-  ensures WFBucketMap(m) ==> WFBucket(bucket)
   ensures BucketWellMarshalled(bucket)
+  ensures |bucket.keys| == |bucket.msgs|
+  ensures WFBucketMap(m) ==> WFBucket(bucket)
+  {
+    BInternalWellMarshalled(m);
+    if WFBucketMap(m) then
+      BInternalWFBucket(m);
+      BInternal(m)
+    else 
+      BInternal(m)
+  }
+
+  function BucketDropLast(bucket: Bucket) : Bucket
+    requires WFBucket(bucket)
+    requires BucketWellMarshalled(bucket)
+    requires 0 < |bucket.keys|
+  {
+    var submap := MapRemove1(bucket.b, Last(bucket.keys));
+    BucketMapWithSeq(submap, DropLast(bucket.keys), DropLast(bucket.msgs))
+  }
+
+  lemma BucketDropLastWF(bucket: Bucket)
+    requires WFBucket(bucket)
+    requires BucketWellMarshalled(bucket)
+    requires 0 < |bucket.keys|
+    ensures WFBucket(BucketDropLast(bucket))
+  {
+    reveal_IsStrictlySorted();
+    reveal_BucketMapOfSeq();
+  }
+
+  lemma BucketDropLastWellMarshalled(bucket: Bucket)
+    requires WFBucket(bucket)
+    requires BucketWellMarshalled(bucket)
+    requires 0 < |bucket.keys|
+    ensures BucketWellMarshalled(BucketDropLast(bucket))
+  {
+    reveal_IsStrictlySorted();
+  }
+
+  
+  lemma WFWellMarshalledBucketMap(bucket: Bucket, key: Key)
+    requires WFBucket(bucket)
+    requires BucketWellMarshalled(bucket)
+    requires key in bucket.b
+    ensures bucket.b[key] == bucket.msgs[LargestLte(bucket.keys, key)]
+    decreases |bucket.keys|
+  {
+    reveal_BucketMapOfSeq();
+    var i :| 0 <= i < |bucket.keys| && bucket.keys[i] == key;
+    PosEqLargestLte(bucket.keys, key, i);
+    if i == |bucket.keys| - 1 {
+      assert bucket.b[key] == Last(bucket.msgs);
+    } else {
+      var bdl := BucketDropLast(bucket);
+      BucketDropLastWF(bucket);
+      BucketDropLastWellMarshalled(bucket);
+      WFWellMarshalledBucketMap(bdl, key);
+    }
+  }
+
+  lemma WFWellMarshalledBucketNoIdentityMsgs(bucket: Bucket)
+    requires WFBucket(bucket)
+    requires BucketWellMarshalled(bucket)
+    ensures IdentityMessage() !in bucket.msgs
+  {
+    forall i | 0 <= i < |bucket.msgs|
+      ensures bucket.msgs[i] != IdentityMessage()
+    {
+      PosEqLargestLte(bucket.keys, bucket.keys[i], i);
+      WFWellMarshalledBucketMap(bucket, bucket.keys[i]);
+    }
+  }
 
   predicate WFBucketAt(bucket: Bucket, pivots: PivotTable, i: int)
   requires WFPivots(pivots)
@@ -68,11 +187,39 @@ module BucketsLib {
   }
 
   lemma WellMarshalledBucketsEq(a: Bucket, b: Bucket)
-  requires BucketWellMarshalled(a)
-  requires BucketWellMarshalled(b)
-  requires a.b == b.b
-  ensures a == b
-
+    requires WFBucket(a)
+    requires WFBucket(b)
+    requires BucketWellMarshalled(a)
+    requires BucketWellMarshalled(b)
+    requires a.b == b.b
+    ensures a == b
+    decreases |a.keys|
+  {
+    if |a.b| == 0 {
+      if 0 < |a.keys| {
+        assert a.keys[0] in Set(a.keys);
+        assert false;
+      }
+      if 0 < |b.keys| {
+        assert b.keys[0] in Set(b.keys);
+        assert false;
+      }
+    } else {
+      var maxkey := Last(a.keys);
+      var maxval := Last(a.msgs);
+      WFWellMarshalledBucketMap(a, maxkey);
+      WFWellMarshalledBucketMap(b, maxkey);
+      
+      var adl := BucketDropLast(a);
+      BucketDropLastWF(a);
+      BucketDropLastWellMarshalled(a);
+      var bdl := BucketDropLast(b);
+      BucketDropLastWF(b);
+      BucketDropLastWellMarshalled(b);
+      WellMarshalledBucketsEq(adl, bdl);
+    }
+  }
+  
   predicate WFBucketList(blist: BucketList, pivots: PivotTable)
   {
     && WFPivots(pivots)
@@ -80,7 +227,6 @@ module BucketsLib {
     && (forall i | 0 <= i < |blist| :: WFBucket(blist[i]))
   }
 
-  // TODO(jonh): suggests rename to ValidlyRoutedBucketList
   predicate WFBucketListProper(blist: BucketList, pivots: PivotTable)
   {
     && WFBucketList(blist, pivots)
@@ -138,7 +284,6 @@ module BucketsLib {
     )
   }
 
-  // TODO(robj&jonh): Can this go away?  Will we ever do unconditionally full flushes?
   function BucketListFlush(parent: Bucket, children: BucketList, pivots: PivotTable) : (res : BucketList)
   requires WFPivots(pivots)
   ensures |res| == |children|
@@ -148,17 +293,6 @@ module BucketsLib {
     BucketListFlushPartial(parent, children, pivots, |children|)
   }
 
-  // TODO(robj): Not yet used, but should replace the complex ensures in BucketMode.partialFlush
-  predicate ValidBucketFlush(oldparent: Bucket, oldchildren: seq<Bucket>,
-    pivots: seq<Key>, newparent: Bucket, newchildren: seq<Bucket>)
-  {
-    && WFBucketListProper(oldchildren, pivots)
-    && WFBucketListProper(newchildren, pivots)
-    && (forall i | 0 <= i < |oldchildren| ::
-      Compose(ClampToSlot(oldparent, pivots, i), oldchildren[i]) ==
-      Compose(ClampToSlot(newparent, pivots, i), newchildren[i]))
-  }
-  
   function JoinBucketList(buckets: seq<Bucket>) : (bucket : Bucket)
   ensures BucketWellMarshalled(bucket)
   {
@@ -168,6 +302,10 @@ module BucketsLib {
   function SplitBucketOnPivots(bucket: Bucket, pivots: seq<Key>) : (buckets: BucketList)
   ensures |buckets| == |pivots| + 1
   ensures BucketListWellMarshalled(buckets)
+  ensures forall i | 0 <= i < |buckets| :: buckets[i].b.Keys <= bucket.b.Keys
+  ensures forall i | 0 <= i < |buckets| :: buckets[i].b.Values <= bucket.b.Values
+  ensures forall i | 0 <= i < |buckets| :: |buckets[i].keys| == |buckets[i].msgs|
+  ensures WFBucketMap(bucket.b) ==> forall i | 0 <= i < |buckets| :: WFBucket(buckets[i])
   decreases |pivots|
   {
     if |pivots| == 0 then (
@@ -202,7 +340,7 @@ module BucketsLib {
   requires WFBucket(bucket)
   ensures WFBucket(BucketIntersect(bucket, keys))
   {
-    reveal_WFBucket();
+    // reveal_WFBucket();
     reveal_BucketIntersect();
   }
 
@@ -210,12 +348,22 @@ module BucketsLib {
   requires WFBucket(bucket)
   ensures WFBucket(BucketComplement(bucket, keys))
   {
-    reveal_WFBucket();
+    // reveal_WFBucket();
     reveal_BucketComplement();
   }
 
   ///// Composeing
 
+  predicate BucketsEquivalentForKey(a: Bucket, b: Bucket, key: Key)
+  {
+    BucketGet(a, key) == BucketGet(b, key)
+  }
+
+  predicate BucketsEquivalent(a: Bucket, b: Bucket)
+  {
+    forall key :: BucketsEquivalentForKey(a, b, key)
+  }
+  
   // Note: does NOT necessarily return a WFBucket!
   // It might contain NoOp messages
   function {:opaque} Compose(top: Bucket, bot: Bucket) : (res : Bucket)
@@ -226,7 +374,7 @@ module BucketsLib {
     :: Merge(BucketGet(top, key), BucketGet(bot, key))
     )
   }
-
+  
   function {:opaque} ComposeSeq(buckets: seq<Bucket>) : (res : Bucket)
   ensures BucketWellMarshalled(res)
   {
@@ -252,11 +400,17 @@ module BucketsLib {
   lemma ComposeAssoc(a: Bucket, b: Bucket, c: Bucket)
   ensures Compose(Compose(a, b), c).b == Compose(a, Compose(b, c)).b
   {
-    assume false;
     reveal_Compose();
-    forall a, b, c ensures Merge(a, Merge(b, c)) == Merge(Merge(a, b), c)
+    var ab_c := Compose(Compose(a, b), c).b;
+    var a_bc := Compose(a, Compose(b, c)).b;
+
+    forall key | key in ab_c.Keys
+      ensures ab_c[key] == a_bc[key]
     {
-      MergeIsAssociative(a, b, c);
+      var av := BucketGet(a, key);
+      var bv := BucketGet(b, key);
+      var cv := BucketGet(c, key);
+      MergeIsAssociative(av, bv, cv);
     }
   }
 
@@ -288,6 +442,17 @@ module BucketsLib {
     }
   }
 
+  predicate FlushEquivalentParentChild(oldparent: Bucket, oldchild: Bucket, newparent: Bucket, newchild: Bucket)
+  {
+    Compose(oldparent, oldchild) == Compose(newparent, newchild)
+  }
+
+  predicate FlushEquivalent(oldparent: Bucket, oldchildren: seq<Bucket>, newparent: Bucket, newchildren: seq<Bucket>)
+  {
+    && |oldchildren| == |newchildren|
+    && (forall i | 0 <= i < |oldchildren| :: FlushEquivalentParentChild(oldparent, oldchildren[i], newparent, newchildren[i]))
+  }
+  
   function InterpretBucketStack(buckets: seq<Bucket>, key: Key) : Message
   {
     if |buckets| == 0 then
@@ -402,12 +567,16 @@ module BucketsLib {
   // NB(jonh): These definitions are timeout monsters.
   function {:opaque} SplitBucketLeft(bucket: Bucket, pivot: Key) : (res : Bucket)
   ensures BucketWellMarshalled(res)
+  ensures |res.keys| == |res.msgs|
+  ensures WFBucketMap(bucket.b) ==> WFBucket(res)
   {
     B(map key | key in bucket.b && Keyspace.lt(key, pivot) :: bucket.b[key])
   }
 
   function {:opaque} SplitBucketRight(bucket: Bucket, pivot: Key) : (res : Bucket)
   ensures BucketWellMarshalled(res)
+  ensures |res.keys| == |res.msgs|
+  ensures WFBucketMap(bucket.b) ==> WFBucket(res)
   {
     B(map key | key in bucket.b && Keyspace.lte(pivot, key) :: bucket.b[key])
   }
@@ -490,7 +659,7 @@ module BucketsLib {
   {
     reveal_SplitBucketLeft();
     WFSlice(pivots, 0, cLeft);
-    reveal_WFBucket();
+    // reveal_WFBucket();
   }
 
   lemma WFProperSplitBucketListLeft(blist: BucketList, pivots: PivotTable, cLeft: int, key: Key)
@@ -520,7 +689,7 @@ module BucketsLib {
   {
     reveal_SplitBucketRight();
     WFSuffix(pivots, cRight);
-    reveal_WFBucket();
+    // reveal_WFBucket();
   }
 
   lemma WFProperSplitBucketListRight(blist: BucketList, pivots: PivotTable, cRight: int, key: Key)
@@ -550,7 +719,23 @@ module BucketsLib {
   ensures WFPivots(insert(pivots, pivot, slot))
   ensures WFBucketList(SplitBucketInList(blist, slot, pivot), insert(pivots, pivot, slot))
   {
-    assume false;
+    WFPivotsInsert(pivots, slot, pivot);
+    reveal_SplitBucketInList();
+    var newbuckets := SplitBucketInList(blist, slot, pivot);
+    forall i | 0 <= i < |newbuckets|
+      ensures WFBucket(newbuckets[i])
+    {
+      if i < slot {
+        assert newbuckets[i] == blist[i];
+      } else if i == slot {
+        reveal_SplitBucketLeft();
+      } else if i == slot + 1 {
+        reveal_SplitBucketRight();
+      } else {
+        assert newbuckets[i] == blist[i-1];
+      }
+    }
+    //WFSplitBucketRight(blist[slot], pivot, pivots, slot);
   }
 
   lemma WFProperSplitBucketInList(blist: BucketList, slot: int, pivot: Key, pivots: PivotTable)
@@ -645,7 +830,7 @@ module BucketsLib {
   requires forall i | 0 <= i < |buckets| :: WFBucket(buckets[i])
   ensures WFBucket(JoinBucketList(buckets))
   {
-    reveal_WFBucket();
+    // reveal_WFBucket();
     if |buckets| == 0 {
     } else {
       WFJoinBucketList(DropLast(buckets));
@@ -675,7 +860,6 @@ module BucketsLib {
   requires WFBucketList(blist, pivots)
   ensures WFBucketList(BucketListFlush(parent, blist, pivots), pivots)
   {
-    assume false;
   }
 
   lemma WFProperBucketListFlush(parent: Bucket, blist: BucketList, pivots: PivotTable)
@@ -888,6 +1072,7 @@ module BucketsLib {
   }
 
   lemma LemmaSplitBucketOnPivotsEqAddMessagesToBuckets(bucket: Bucket, pivots: seq<Key>, emp: seq<Bucket>)
+  requires WFBucket(bucket)
   requires WFPivots(pivots)
   requires |emp| == |pivots| + 1
   requires forall i | 0 <= i < |emp| :: emp[i] == B(map[])
@@ -936,7 +1121,7 @@ module BucketsLib {
   requires WFPivots(pivots)
   ensures WFBucketListProper(SplitBucketOnPivots(bucket, pivots), pivots)
   {
-    reveal_WFBucket();
+    // reveal_WFBucket();
     var e := emptyList(|pivots| + 1);
     LemmaSplitBucketOnPivotsEqAddMessagesToBuckets(bucket, pivots, e);
     WFBucketListFlush(bucket, e, pivots);
@@ -950,7 +1135,7 @@ module BucketsLib {
   decreases |pivots|
   {
     WFSplitBucketOnPivots(bucket, pivots);
-    reveal_WFBucket();
+    // reveal_WFBucket();
 
     if |pivots| == 0 {
     } else {
@@ -993,7 +1178,7 @@ module BucketsLib {
   requires 1 <= i <= |blist|
   ensures WFBucketList(blist[.. i], pivots[.. i-1])
   {
-    assume false;
+    StrictlySortedSubsequence(pivots, 0, i-1);
   }
 
   lemma WFBucketListSplitRight(blist: BucketList, pivots: PivotTable, i: int)
@@ -1001,7 +1186,12 @@ module BucketsLib {
   requires 0 <= i < |blist|
   ensures WFBucketList(blist[i ..], pivots[i ..])
   {
-    assume false;
+    assert pivots[i..] == pivots[i..|pivots|];
+    StrictlySortedSubsequence(pivots, i, |pivots|);
+    if 0 < i < |pivots| {
+      IsStrictlySortedImpliesLt(pivots, 0, i);
+      IsNotMinimum(pivots[0], pivots[i]);
+    }
   }
 
   lemma WFProperBucketListSplitLeft(blist: BucketList, pivots: PivotTable, i: int)
@@ -1044,15 +1234,49 @@ module BucketsLib {
     }
   }
 
+  function binarySearch(keys: seq<Key>, key: Key) : (i : Option<nat>)
+    ensures IsStrictlySorted(keys) ==> i.None? ==> key !in keys
+    ensures i.Some? ==> 0 <= i.value < |keys| && key == keys[i.value]
+  {
+    if |keys| == 0 then
+      None
+    else
+      reveal_IsStrictlySorted();
+      var mid := |keys| / 2;
+      if lt(key, keys[mid]) then
+        binarySearch(keys[..mid], key)
+      else if keys[mid] == key then
+        Some(mid)
+      else
+        var sub := binarySearch(keys[mid+1..], key);
+        if sub.Some? then
+          Some(mid + 1 + sub.value)
+        else
+          None
+  }
+  
   // This binary searches on the keys list in bucket.
   // If it happens to be in sorted order, it will return the correct
   // answer.
   function bucketBinarySearchLookup(bucket: Bucket, key: Key)
     : (msg : Option<Message>)
-  ensures BucketWellMarshalled(bucket) ==> msg.None? ==> key !in bucket.b
-  ensures BucketWellMarshalled(bucket) ==> msg.Some? ==>
+    requires WFBucket(bucket)
+    ensures BucketWellMarshalled(bucket) ==> msg.None? ==> key !in bucket.b
+    ensures BucketWellMarshalled(bucket) ==> msg.Some? ==>
       key in bucket.b && bucket.b[key] == msg.value
-
+  {
+    var i := binarySearch(bucket.keys, key);
+    if i.Some? then 
+      (if BucketWellMarshalled(bucket) then
+        WFWellMarshalledBucketMap(bucket, key);
+        PosEqLargestLte(bucket.keys, key, i.value);
+        Some(bucket.msgs[i.value])
+      else
+        Some(bucket.msgs[i.value]))
+    else
+      None
+  }
+  
   function getMiddleKey(bucket: Bucket) : Key
   requires WFBucket(bucket)
   {
@@ -1066,4 +1290,5 @@ module BucketsLib {
         key
     )
   }
+
 }
